Subtype Reflexivity and Membership wf

type_members/ftfjp2018/coq/vars.v
@@ -393,14 +393,459 @@ Proof.
     auto.
 Qed.
 
+Definition unbound_in_dty := strengthening_utils.unbound_in_dty.
+
 Lemma struct_contains_wf :
   forall Sig G t, Sig en G vdash t wf_t ->
+           Sig wf_st ->
+           Sig evdash G wf_env ->
            forall s, s cont_w t ->
                 forall p, Sig en G vdash p pathType t ->
-                     Sig en t::G vdash [p /s 0]s wf_s.
+                     Sig en G vdash p wf_e ->
+                     Sig en G vdash [p /s 0]s wf_s.
 Proof.
   intros.
+  inversion H2; subst.
+  inversion H; subst.
+  apply subst_in_dty
+    with
+      (p:=c_ (length G))(n:=0)
+    in H5.
+  apply in_dty_wf
+    with
+      (Sig:=Sig)(G:=str ss::G)
+    in H5;
+    auto.
+  apply wf_subst_decl_ty_actual
+    with
+      (p:=p)
+    in H5;
+    auto.
+
+  apply wf_con;
+    auto.
   
-  
+  apply unbound_in_dty with (ss:=ss);
+    inversion H2;
+    auto.
 Qed.
+
+Lemma path_typing_wf :
+  forall Sig G p t, Sig en G vdash p pathType t ->
+             Sig wf_st ->
+             Sig evdash G wf_env ->
+             Sig en G vdash p wf_e ->
+             Sig en G vdash t wf_t.
+Proof.
+  intros Sig G p t Htyp;
+    induction Htyp;
+    intros;
+    auto.
+
+  apply wf_in_env;
+    auto.
+  eapply in_rev, get_in;
+    eauto.
+
+  apply wf_in_store_type;
+    auto.
+  eapply in_rev, get_in;
+    eauto.
+
+  inversion H2;
+    eauto.
+Qed.
+
+Scheme type_mutind' := Induction for ty Sort Prop
+  with decl_ty_mutind' := Induction for decl_ty Sort Prop
+  with decl_tys_mutind' := Induction for decl_tys Sort Prop.
+
+Combined Scheme type_mutind from type_mutind', decl_ty_mutind', decl_tys_mutind'.
+
+Fixpoint raise_list (E : list exp) : list exp :=
+  match E with
+  | nil => nil
+  | e :: E' => (e raise_e 0)::(raise_list E')
+  end.
+
+Fixpoint lsubst_t (E : list exp)(n : nat)(t : ty) : ty :=
+  match E with
+  | nil => t
+  | e :: E' => [e /t n](lsubst_t E' (S n) t)
+  end.
+
+Fixpoint lsubst_s (E : list exp)(n : nat)(s : decl_ty) : decl_ty :=
+  match E with
+  | nil => s
+  | e :: E' => [e /s n](lsubst_s E' (S n) s)
+  end.
+
+Fixpoint lsubst_ss (E : list exp)(n : nat)(ss : decl_tys) : decl_tys :=
+  match E with
+  | nil => ss
+  | e :: E' => [e /ss n](lsubst_ss E' (S n) ss)
+  end.
+
+Fixpoint lsubst_e (E : list exp)(n : nat)(e : exp) : exp :=
+  match E with
+  | nil => e
+  | e' :: E' => [e' /e n](lsubst_e E' (S n) e)
+  end.
+
+Fixpoint lsubst_d (E : list exp)(n : nat)(d : decl) : decl :=
+  match E with
+  | nil => d
+  | e :: E' => [e /d n](lsubst_d E' (S n) d)
+  end.
+
+Fixpoint lsubst_ds (E : list exp)(n : nat)(ds : decls) : decls :=
+  match E with
+  | nil => ds
+  | e :: E' => [e /ds n](lsubst_ds E' (S n) ds)
+  end.
+
+Lemma lsubst_ty_sel :
+  forall E n p l, (lsubst_t E n (sel p l)) = (sel (lsubst_e E n p) l).
+Proof.
+  intros E;
+    induction E as [|e' E'];
+    intros;
+    auto.
   
+  simpl;
+    rewrite IHE';
+    auto.
+Qed.
+
+Hint Rewrite lsubst_ty_sel.
+Hint Resolve lsubst_ty_sel.
+
+Lemma lsubst_ty_top :
+  forall E n, (lsubst_t E n top) = top.
+Proof.
+  intro E;
+    induction E;
+    auto;
+    intros;
+    simpl;
+    rewrite IHE;
+    auto.
+Qed.
+
+Hint Rewrite lsubst_ty_top.
+Hint Resolve lsubst_ty_top.
+
+Lemma lsubst_ty_bot :
+  forall E n, (lsubst_t E n bot) = bot.
+Proof.
+  intro E;
+    induction E;
+    auto;
+    intros;
+    simpl;
+    rewrite IHE;
+    auto.
+Qed.
+
+Hint Rewrite lsubst_ty_bot.
+Hint Resolve lsubst_ty_bot.
+
+Lemma lsubst_ty_arr :
+  forall E n t1 t2, (lsubst_t E n (t1 arr t2)) = ((lsubst_t E n t1) arr (lsubst_t (raise_list E) (S n) t2)).
+Proof.
+  intro E;
+    induction E as [|e E'];
+    intros;
+    auto;
+    simpl.
+  
+  rewrite IHE'; 
+    auto.
+Qed.
+
+Hint Rewrite lsubst_ty_arr.
+Hint Resolve lsubst_ty_arr.
+
+Lemma lsubst_ty_str :
+  forall E n ss, (lsubst_t E n (str ss)) = (str (lsubst_ss (raise_list E) (S n) ss)).
+Proof.
+  intro E;
+    induction E as [|e' E'];
+    intros;
+    simpl;
+    auto.
+
+  rewrite IHE';
+    auto.
+Qed.
+
+Hint Rewrite lsubst_ty_str.
+Hint Resolve lsubst_ty_str.
+
+Lemma lsubst_decl_ty_upper :
+  forall E n l t, (lsubst_s E n (type l ext t)) = (type l ext (lsubst_t E n t)).
+Proof.
+  intros E;
+    induction E as [|e' E'];
+    intros;
+    auto.
+  
+  simpl;
+    rewrite IHE';
+    auto.
+Qed.
+
+Hint Rewrite lsubst_decl_ty_upper.
+Hint Resolve lsubst_decl_ty_upper.
+
+Lemma lsubst_decl_ty_lower :
+  forall E n l t, (lsubst_s E n (type l sup t)) = (type l sup (lsubst_t E n t)).
+Proof.
+  intros E;
+    induction E as [|e' E'];
+    intros;
+    auto.
+  
+  simpl;
+    rewrite IHE';
+    auto.
+Qed.
+
+Hint Rewrite lsubst_decl_ty_lower.
+Hint Resolve lsubst_decl_ty_lower.
+
+Lemma lsubst_decl_ty_equal :
+  forall E n l t, (lsubst_s E n (type l eqt t)) = (type l eqt (lsubst_t E n t)).
+Proof.
+  intros E;
+    induction E as [|e' E'];
+    intros;
+    auto.
+  
+  simpl;
+    rewrite IHE';
+    auto.
+Qed.
+
+Hint Rewrite lsubst_decl_ty_equal.
+Hint Resolve lsubst_decl_ty_equal.
+
+Lemma lsubst_decl_ty_value :
+  forall E n l t, (lsubst_s E n (val l oft t)) = (val l oft (lsubst_t E n t)).
+Proof.
+  intros E;
+    induction E as [|e' E'];
+    intros;
+    auto.
+  
+  simpl;
+    rewrite IHE';
+    auto.
+Qed.
+
+Hint Rewrite lsubst_decl_ty_value.
+Hint Resolve lsubst_decl_ty_value.
+
+Lemma lsubst_nil :
+  forall E n, (lsubst_ss E n (dt_nil)) = dt_nil.
+Proof.
+  intro E;
+    induction E as [|e E'];
+    intros;
+    auto;
+    simpl.
+  
+  rewrite IHE'; 
+    auto.
+Qed.
+
+Hint Rewrite lsubst_nil.
+Hint Resolve lsubst_nil.
+
+Lemma lsubst_decl_tys_con :
+  forall E n s ss, (lsubst_ss E n (dt_con s ss)) = (dt_con (lsubst_s E n s) (lsubst_ss E n ss)).
+Proof.
+  intro E;
+    induction E as [|e E'];
+    intros;
+    auto;
+    simpl.
+  
+  rewrite IHE'; 
+    auto.
+Qed.
+
+Hint Rewrite lsubst_decl_tys_con.
+Hint Resolve lsubst_decl_tys_con.
+
+
+Lemma subtype_reflexivity_mutind :
+  (forall t E Sig G1 G2, length G1 = length G2 -> Sig en G1 vdash (lsubst_t E 0 t) <; (lsubst_t E 0 t) dashv G2) /\
+  (forall s E Sig G1 G2, length G1 = length G2 -> Sig en G1 vdash (lsubst_s E 0 s) <;; (lsubst_s E 0 s) dashv G2) /\
+  (forall ss E Sig G1 G2, length G1 = length G2 -> Sig en G1 vdash (lsubst_ss E 0 ss) <;;; (lsubst_ss E 0 ss) dashv G2).
+Proof.
+  apply type_mutind;
+    intros;
+    simpl;
+    auto;
+    try solve [rewrite lsubst_ty_sel;
+               auto];
+    try solve [rewrite lsubst_ty_top;
+               auto];
+    try solve [rewrite lsubst_ty_bot;
+               auto];
+    try solve [rewrite lsubst_decl_ty_upper;
+               auto];
+    try solve [rewrite lsubst_decl_ty_lower;
+               auto];
+    try solve [rewrite lsubst_decl_ty_equal;
+               auto];
+    try solve [rewrite lsubst_decl_ty_value;
+               auto];
+    try solve [rewrite lsubst_nil;
+               auto];
+    try solve [rewrite lsubst_decl_tys_con;
+               auto].
+
+  (*str*)
+  rewrite lsubst_ty_str.
+  apply s_struct with (i:= length G1);
+    auto;
+    simpl.
+  assert (Hsub : (length (str (lsubst_ss (raise_list E) 1 d) :: G1)) =
+                 (length (str (lsubst_ss (raise_list E) 1 d) :: G2)));
+    [simpl
+    |apply H
+       with
+         (E:=(c_ (length G1))::(raise_list E))
+         (Sig:=Sig)
+      in Hsub;
+    simpl in Hsub];
+    auto.
+
+  (*arr*)
+  rewrite lsubst_ty_arr.
+  apply s_arr with (i:=length G1);
+    auto;
+    simpl.
+  assert (Hsub : (length ((lsubst_t E 0 t) :: G1)) =
+                 (length ((lsubst_t E 0 t) :: G2)));
+    [simpl
+    |apply H0
+       with
+         (E:=(c_ (length G1))::(raise_list E))
+         (Sig:=Sig)
+      in Hsub;
+    simpl in Hsub];
+    auto.
+Qed.
+
+Lemma subtype_reflexivity :
+  forall Sig G1 t G2, length G1 = length G2 ->
+               Sig en G1 vdash t <; t dashv G2.
+Proof.
+  intros.
+  destruct subtype_reflexivity_mutind as [Ha Hb].
+  apply Ha
+    with
+      (t:=t)
+      (E:=nil)
+      (Sig:=Sig)
+    in H;
+    simpl in Ha;
+    auto.
+Qed.
+
+Lemma alt_has_wf :
+  (forall Sig G p s, Sig en G vdash p ni_w s ->
+              Sig wf_st ->
+              Sig evdash G wf_env ->
+              Sig en G vdash p wf_e ->
+              Sig en G vdash s wf_s).
+Proof.
+  intros Sig G p s Hni;
+    induction Hni;
+    intros;
+    auto.
+
+  (*struct*)
+  apply struct_contains_wf with (t:=str ss);
+    auto.
+  eapply path_typing_wf;
+    eauto.
+
+  (*upper*)
+  apply IHHni2;
+    auto.
+  assert (HwfSel : Sig en G vdash sel p' l' wf_t);
+    [apply path_typing_wf in H;
+     auto|].
+  assert (Hwfp' : Sig en G vdash p' wf_e);
+    [inversion HwfSel;
+     auto
+    |].
+  assert (HwfUpper : Sig en G vdash type l' ext t wf_s);
+    [apply IHHni1;
+     auto;
+     inversion HwfSel;
+     auto
+    |].
+  apply wf_cast with (t':=sel p' l');
+    eauto;
+    [inversion HwfUpper;
+     auto
+    |apply path_typing_implies_typing;
+     auto
+    |].
+  apply s_upper with (t1:=t);
+    auto.
+  apply alt_has_implies_has;
+    auto.
+  intros n' Hle;
+    eapply wf_closed_exp;
+    eauto.
+  apply wf_closed_store_type;
+    auto.
+  eapply wf_closed_env;
+    eauto.
+  apply subtype_reflexivity;
+    auto.
+
+  (*equal*)
+  apply IHHni2;
+    auto.
+  assert (HwfSel : Sig en G vdash sel p' l' wf_t);
+    [apply path_typing_wf in H;
+     auto|].
+  assert (Hwfp' : Sig en G vdash p' wf_e);
+    [inversion HwfSel;
+     auto
+    |].
+  assert (HwfEqual : Sig en G vdash type l' eqt t wf_s);
+    [apply IHHni1;
+     auto;
+     inversion HwfSel;
+     auto
+    |].
+  apply wf_cast with (t':=sel p' l');
+    eauto;
+    [inversion HwfEqual;
+     auto
+    |apply path_typing_implies_typing;
+     auto
+    |].
+  apply s_equal1 with (t1:=t);
+    auto.
+  apply alt_has_implies_has;
+    auto.
+  intros n' Hle;
+    eapply wf_closed_exp;
+    eauto.
+  apply wf_closed_store_type;
+    auto.
+  eapply wf_closed_env;
+    eauto.
+  apply subtype_reflexivity;
+    auto.
+Qed.
+
